Started working on eps-NFA -> NFA conversion

src/automata/epsnfa.lean
@@ -2,18 +2,181 @@ import data.set.basic
 import data.set.finite
 import automata.nfa
 
-open set nfa
+open set
 
 namespace epsnfa
 
 variables {S Q : Type}
-
 
 structure epsNFA (S : Type) (Q : Type) :=
     (start : Q) -- starting state
     (term : set Q) -- terminal states
     (next : Q → S → set Q) -- transitions
     (eps : Q → set Q) -- eps-transitions
+
+inductive go (enfa : epsNFA S Q) : Q → list S → Q → Prop
+| finish : Π {q : Q}, go q [] q
+| step   : Π {head : S} {tail : list S} {q n f : Q} (h : n ∈ enfa.next q head),
+    go n tail f → go q (head::tail) f 
+| eps    : Π {tail : list S} {q n f : Q} (h : n ∈ enfa.eps q),
+    go n tail f → go q tail f
+
+@[simp] def epsnfa_accepts_word (enfa : epsNFA S Q) (w : list S) : Prop := 
+    ∃ {t}, go enfa enfa.start w t ∧ t ∈ enfa.term
+
+@[simp] def lang_of_epsnfa (enfa : epsNFA S Q) := {w | epsnfa_accepts_word enfa w}
+
+def epsnfa_lang (lang : set (list S)) : Prop := 
+    ∃ {Q : Type} (enfa : epsNFA S Q), lang = lang_of_epsnfa enfa
+
+lemma epsnfa_go_trans {enfa : epsNFA S Q} {a b c : Q} {left right : list S}:
+    go enfa a left b → go enfa b right c → go enfa a (left ++ right) c :=
+begin
+    rintro hab hfc,
+    induction hab with q  head tail q n f h prev ih  tail q n f h prev ih, 
+    { exact hfc }, 
+    { apply go.step h (ih hfc) },
+    { apply go.eps h (ih hfc) },
+end
+
+lemma epsnfa_go_exists_trans {enfa : epsNFA S Q} {a c : Q} 
+    {left right concat : list S} {clr : left ++ right = concat}:
+    go enfa a concat c → (∃ {b : Q}, go enfa a left b ∧ go enfa b right c) :=
+begin
+    intros go_ac,
+    induction go_ac with q  head tail q n f h prev ih  tail q n f h prev ih generalizing left, {
+        rw list.append_eq_nil at clr,
+        rcases clr with ⟨rfl, rfl⟩,
+        use [q, go.finish, go.finish],
+    }, {
+        by_cases left_nil : (left = []), {
+            subst left_nil,
+            dsimp at clr,
+            subst clr,
+            specialize @ih [],
+            use [q, go.finish, go.step h prev],
+        }, {
+            cases left, contradiction,
+            rw [list.cons_append, list.cons.inj_eq] at clr,
+            rcases clr with ⟨rfl, rfl⟩,
+            rcases @ih left_tl rfl with ⟨b, goleft, goright⟩,
+            use [b, go.step h goleft, goright],
+        }
+    }, {
+        subst clr,
+        rcases @ih left rfl with ⟨b, goleft, goright⟩,
+        use [b, go.eps h goleft, goright],
+    }
+end
+
+def eps_reach (enfa : epsNFA S Q) (q : Q) (r : Q) := go enfa q [] r
+
+def epsnfa_to_nfa (enfa : epsNFA S Q) : nfa.NFA S Q := {
+    start := enfa.start,
+    term := {x | ∃ t, eps_reach enfa x t ∧ t ∈ enfa.term},
+    next := λ q c, {r | ∃ x y, eps_reach enfa q x ∧ y ∈ enfa.next x c ∧ eps_reach enfa y r}
+}
+
+lemma epsnfa_to_nfa_singleton (en : epsNFA S Q) {n : nfa.NFA S Q} (w : S) (s1 e1 : Q)
+    : (n = epsnfa_to_nfa en) → (go en s1 [w] e1 ↔ nfa.go n s1 [w] e1) :=
+begin
+    rintro enfa_nfa,
+    split, {
+        intro go_enfa,
+        induction go_enfa, {
+            exact nfa.go.finish,
+        }, {
+            rcases go_enfa_ih with ⟨_⟩, {
+                sorry,
+            }, {
+                sorry,
+            }
+        }, {
+            sorry,
+        }
+    }, {
+        subst enfa_nfa,
+        -- dsimp [epsnfa_to_nfa] at *,
+        rintro (_ | ⟨head, tail, q, n, f, h, go_nil⟩),
+        rcases go_nil,
+        rcases h with ⟨x, y, eps_s1x, ynext, eps_yn⟩,
+        exact epsnfa_go_trans eps_s1x (go.step ynext eps_yn),
+    }
+end
+
+lemma epsnfa_to_nfa_goes_to     
+    (en : epsNFA S Q) {n : nfa.NFA S Q} (w : list S) (s1 e1 : Q)
+    : (n = epsnfa_to_nfa en) → (w ≠ []) → (go en s1 w e1 ↔ nfa.go n s1 w e1) :=
+begin
+    rintro enfa_nfa,
+    induction w with fst tail hyp generalizing s1, {
+        tauto!,
+    }, {
+        rcases tail with _ | ⟨snd, rest⟩, {
+            rintro hdnil,
+            clear hdnil hyp,
+            refine epsnfa_to_nfa_singleton _ _ _ _ enfa_nfa,
+        }, {
+            intro h, clear h,
+            split, {
+                intro go_enfa,
+                rcases go_enfa with ⟨_⟩ | ⟨_, _, _, nxt, _, hnxt, prev⟩ | ⟨_, _, nxt, _, hnxt, prev⟩, {
+                    specialize @hyp nxt (list.cons_ne_nil _ _),
+                    replace hyp := hyp.1 prev,
+                    refine @nfa.go.step _ _ _ _ _ _ nxt _ _ hyp,
+                    subst enfa_nfa,
+                    use [s1, nxt, go.finish, hnxt, go.finish],
+                }, {
+                    specialize @hyp nxt (list.cons_ne_nil _ _),
+                    sorry,
+                },
+            }, {
+                sorry,
+            }
+        }
+    }
+end
+
+theorem epsnfa_to_nfa_eq {L : set (list S)} : epsnfa_lang L → nfa.nfa_lang L :=
+begin
+    rintro ⟨Q, enf, rfl⟩,
+    use [Q, epsnfa_to_nfa enf],
+    ext x,
+    dsimp,
+    split, {
+        rintro ⟨t, tgo, tterm⟩,
+        by_cases (x = []), {
+            subst h,
+            use enf.start,
+            split,
+            use [nfa.go.finish],
+            use [t, tgo, tterm],
+        }, {
+            use t,
+            have tmp := epsnfa_to_nfa_goes_to enf x (epsnfa_to_nfa enf).start t rfl h,
+            rw ← tmp,
+            use [tgo, t, epsnfa.go.finish, tterm], 
+        }
+    }, {
+        rintro ⟨t, tgo, tterm⟩,
+        by_cases xnil : x = [], {
+            subst xnil,
+            cases tgo,
+            use tterm,
+        }, {
+            rcases tterm with ⟨endt, endt_epsreach, endt_term⟩,
+            use endt,
+            have tmp := epsnfa_to_nfa_goes_to enf x (epsnfa_to_nfa enf).start t rfl xnil,
+            rw ← tmp at tgo,
+            split, {
+                convert epsnfa_go_trans tgo endt_epsreach,
+                simp only [list.append_nil], 
+            }, {
+                exact endt_term,
+            }
+        }
+    }
+end
 
 
 end epsnfa
